add trace digest combine and reaching_compat witnesses

src/CFG/Collecting/CFG_Collect_Trace.thy
@@ -1,5 +1,5 @@
 theory CFG_Collect_Trace
-  imports CFG_Collect "Voblint_IMP2.IMP2_Globals"
+  imports CFG_Collect_Runs "Voblint_IMP2.IMP2_Globals"
 begin
 
 section \<open>Trace-valued collecting semantics\<close>
@@ -55,11 +55,22 @@ lemma alpha_last_mono:
   "A \<subseteq> B \<Longrightarrow> alpha_last A \<subseteq> alpha_last B"
   unfolding alpha_last_def by blast
 
+subsection \<open>Procedure entry points\<close>
+
+definition proc_entry_pps :: "cfg \<Rightarrow> pp set" where
+  "proc_entry_pps g = {v. \<exists>u. (u, EA_Enter, v) \<in> edges g}"
+
+lemma proc_entry_ppsI:
+  "(u, EA_Enter, v) \<in> edges g \<Longrightarrow> v \<in> proc_entry_pps g"
+  unfolding proc_entry_pps_def by blast
+
 subsection \<open>Interprocedural trace witness\<close>
 
 text \<open>
   trace_witness g S v tr : tr is a store sequence reaching v.
   entry   : a singleton [s] for s in the initial set, at the CFG entry.
+  proc_entry : callee-relative seed [s] at procedure entry pp when the CFG
+            has an enter edge from cfg_entry (call-at-main-entry layout).
   edge    : extend by one CFG edge (covers intra edges AND enter edges, since
             EA_Enter is an ordinary edge_action with edge_step EA_Enter s =
             Some (enter_state s)).
@@ -71,6 +82,8 @@ text \<open>
 \<close>
 inductive trace_witness :: "cfg \<Rightarrow> store set \<Rightarrow> pp \<Rightarrow> trace \<Rightarrow> bool" for g S where
   entry: "v = cfg_entry g \<Longrightarrow> s \<in> S \<Longrightarrow> trace_witness g S v [s]"
+| proc_entry:
+    "(cfg_entry g, EA_Enter, v) \<in> edges g \<Longrightarrow> s \<in> enter_state ` S \<Longrightarrow> trace_witness g S v [s]"
 | edge: "(u, a, v) \<in> edges g \<Longrightarrow> trace_witness g S u tr
          \<Longrightarrow> edge_step a (last tr) = Some s'
          \<Longrightarrow> trace_witness g S v (tr @ [s'])"
@@ -89,9 +102,157 @@ lemma trace_witness_nonempty:
   "trace_witness g S v tr \<Longrightarrow> tr \<noteq> []"
   by (induction rule: trace_witness.induct) auto
 
+lemma trace_witness_mono_initial:
+  assumes "S' \<subseteq> S"
+  assumes "trace_witness g S' v tr"
+  shows "trace_witness g S v tr"
+  using assms(2)
+proof (induction rule: trace_witness.induct)
+  case (entry v s)
+  then show ?case using entry assms(1) by (auto intro!: trace_witness.entry)
+next
+  case (proc_entry v s)
+  then show ?case using proc_entry assms(1) by (auto intro!: trace_witness.proc_entry)
+next
+  case (edge u a v tr s')
+  then show ?case by (auto intro!: trace_witness.intros)
+next
+  case (combine c ex v tau \<rho>)
+  then show ?case by (auto intro!: trace_witness.intros)
+qed
+
+lemma proc_entry_pps_mono:
+  "edges g' \<subseteq> edges g \<Longrightarrow> proc_entry_pps g' \<subseteq> proc_entry_pps g"
+  by (auto simp: proc_entry_pps_def)
+
+lemma trace_witness_ext_edges:
+  assumes edge_sub: "edges g' \<subseteq> edges g"
+  assumes comb_sub: "combines g' \<subseteq> combines g"
+  assumes entry_eq: "cfg_entry g = cfg_entry g'"
+  assumes w: "trace_witness g' S v tr"
+  shows "trace_witness g S v tr"
+  using w
+proof (induction rule: trace_witness.induct)
+  case (entry v s)
+  then show ?case using entry_eq by (auto intro!: trace_witness.entry)
+next
+  case (proc_entry v s)
+  then have enter': "(cfg_entry g', EA_Enter, v) \<in> edges g'" by simp
+  have enter: "(cfg_entry g, EA_Enter, v) \<in> edges g"
+    using edge_sub enter' entry_eq by auto
+  then show ?case using proc_entry.hyps(2) enter
+    by (intro trace_witness.proc_entry)
+next
+  case (edge u a v tr s')
+  then show ?case
+    using edge_sub edge.hyps(1) edge.IH
+    by (auto intro!: trace_witness.intros)
+next
+  case (combine c ex v tau \<rho>)
+  then show ?case
+    using comb_sub combine.hyps(1) combine.IH
+    by (auto intro!: trace_witness.intros)
+qed
+
+lemma trace_witness_assign_from_entry_store:
+  fixes g :: cfg and S :: "store set" and ent body :: store and u v :: pp
+    and x :: vname and a :: aexp
+  assumes ent_in: "ent \<in> S"
+  assumes proc_ent: "u = cfg_entry g"
+  assumes edge: "(u, EA_Assign x a, v) \<in> edges g"
+  assumes body: "body = ent(x := aval a ent)"
+  shows "trace_witness g S v [ent, body]"
+proof -
+  have ent_w: "trace_witness g S (cfg_entry g) [ent]"
+    using ent_in by (intro trace_witness.entry) simp
+  have ent_w': "trace_witness g S u [ent]"
+    using ent_w proc_ent by simp
+  show ?thesis
+    using body ent_w' local.edge trace_witness.edge by fastforce
+qed
+
+lemma trace_witness_assign_from_proc_entry:
+  fixes g :: cfg and S :: "store set" and ent body :: store and pe ex :: pp
+    and x :: vname and a :: aexp
+  assumes ent_in: "ent \<in> enter_state ` S"
+  assumes enter_edge: "(cfg_entry g, EA_Enter, pe) \<in> edges g"
+  assumes edge: "(pe, EA_Assign x a, ex) \<in> edges g"
+  assumes body: "body = ent(x := aval a ent)"
+  shows "trace_witness g S ex [ent, body]"
+proof -
+  have ent_w: "trace_witness g S pe [ent]"
+    using ent_in enter_edge by (intro trace_witness.proc_entry) simp
+  show ?thesis
+    using body ent_w edge trace_witness.edge by fastforce
+qed
+
 lemma cfg_collect_trace_entry:
   "s \<in> S \<Longrightarrow> [s] \<in> cfg_collect_trace g S (cfg_entry g)"
   unfolding cfg_collect_trace_def using trace_witness.entry by simp
+
+
+subsection \<open>Linear edge traces\<close>
+
+inductive trace_edges :: "cfg => pp => trace => pp => bool" for g where
+  single: "trace_edges g v [s] v"
+| step:
+    "trace_edges g u tr v
+     ==> (v, a, w) \<in> edges g
+     ==> edge_step a (last tr) = Some s'
+     ==> trace_edges g u (tr @ [s']) w"
+
+lemma trace_edges_nonempty:
+  "trace_edges g u tr v ==> tr \<noteq> []"
+  by (induction rule: trace_edges.induct) auto
+
+lemma trace_witness_edges:
+  assumes path: "trace_edges g u tr v"
+  assumes start: "u = cfg_entry g"
+  assumes init: "hd tr \<in> S"
+  shows "trace_witness g S v tr"
+  using path start init
+proof (induction rule: trace_edges.induct)
+  case (single v s)
+  then show ?case by (intro trace_witness.entry) auto
+next
+  case (step u tr v a w s')
+  have tr_ne: "tr \<noteq> []"
+    using step.hyps(1) by (rule trace_edges_nonempty)
+  have prev: "trace_witness g S v tr"
+    using step.IH step.prems(1,2) tr_ne by simp
+  show ?case
+    using trace_witness.edge[OF step.hyps(2) prev step.hyps(3)] by simp
+qed
+
+lemma trace_witness_proc_edges:
+  assumes enter: "(cfg_entry g, EA_Enter, pe) \<in> edges g"
+  assumes path: "trace_edges g u tr v"
+  assumes start: "u = pe"
+  assumes init: "hd tr \<in> enter_state ` S"
+  shows "trace_witness g S v tr"
+  using path start init
+proof (induction rule: trace_edges.induct)
+  case (single v s)
+  then show ?case using enter by (intro trace_witness.proc_entry) auto
+next
+  case (step u tr v a w s')
+  have tr_ne: "tr \<noteq> []"
+    using step.hyps(1) by (rule trace_edges_nonempty)
+  have prev: "trace_witness g S v tr"
+    using step.IH step.prems(1,2) tr_ne by simp
+  show ?case
+    using trace_witness.edge[OF step.hyps(2) prev step.hyps(3)] by simp
+qed
+
+
+lemma trace_witness_combineI:
+  assumes comb: "(c, ex, v) \<in> combines g"
+  assumes caller: "trace_witness g S c tau"
+  assumes callee: "trace_witness g S ex rho"
+  assumes enter: "hd rho = enter_state (last tau)"
+  assumes ret: "r = <last tau|last rho>"
+  shows "trace_witness g S v (tau @ tl rho @ [r])"
+  using assms trace_witness.combine by fastforce
 
 subsection \<open>Interprocedural projection\<close>
 
@@ -100,6 +261,34 @@ text \<open>
   interprocedural collecting.  Carries traces through the same lfp post-fixpoint
   steps as cfg_witness_in_cfg_collect (CFG_Collect), projecting with last.
 \<close>
+
+lemma enter_state_mem_cfg_collect_proc_entry:
+  assumes enter: "(u, EA_Enter, pe) \<in> edges g"
+  assumes sub: "S \<subseteq> cfg_collect g S u"
+  assumes s: "s \<in> enter_state ` S"
+  shows "s \<in> cfg_collect g S pe"
+proof -
+  obtain s' where s'_in: "s' \<in> S" and s_eq: "s = enter_state s'"
+    using s by blast
+  have "s' \<in> cfg_collect g S u" using sub s'_in by blast
+  have ent_in: "s \<in> edge_collect EA_Enter (cfg_collect g S u)"
+    using s_eq `s' \<in> cfg_collect g S u` by force
+  show ?thesis using cfg_collect_edge[OF enter ent_in] by simp
+qed
+
+lemma enter_state_image_subset_cfg_collect_proc_entry:
+  assumes enter: "(cfg_entry g, EA_Enter, pe) \<in> edges g"
+  shows "enter_state ` S \<subseteq> cfg_collect g S pe"
+proof
+  fix s
+  assume s_in: "s \<in> enter_state ` S"
+  then obtain s' where s'_in: "s' \<in> S" and s_eq: "s = enter_state s'"
+    by blast
+  show "s \<in> cfg_collect g S pe"
+    using enter_state_mem_cfg_collect_proc_entry[OF enter cfg_collect_entry s_in]
+    by simp
+qed
+
 lemma trace_witness_last_in_cfg_collect:
   assumes "trace_witness g S v tr"
   shows "last tr \<in> cfg_collect g S v"
@@ -107,6 +296,13 @@ lemma trace_witness_last_in_cfg_collect:
 proof (induction rule: trace_witness.induct)
   case (entry v s)
   then show ?case using cfg_collect_entry by auto
+next
+  case (proc_entry v s)
+  then have sub: "enter_state ` S \<subseteq> cfg_collect g S v"
+    using enter_state_image_subset_cfg_collect_proc_entry[OF proc_entry.hyps(1)]
+    by simp
+  then show ?case
+    using proc_entry.hyps(2) sub by (auto simp: subset_iff)
 next
   case (edge u a v tr s')
   have ih: "last tr \<in> cfg_collect g S u" using edge.IH .
@@ -156,6 +352,8 @@ inductive trace_witness_d ::
   "(trace \<Rightarrow> 'd) \<Rightarrow> ('d \<Rightarrow> 'd \<Rightarrow> bool) \<Rightarrow> cfg \<Rightarrow> store set \<Rightarrow> pp \<Rightarrow> trace \<Rightarrow> bool"
   for dg :: "trace \<Rightarrow> 'd" and cmp :: "'d \<Rightarrow> 'd \<Rightarrow> bool" and g S where
   entry: "v = cfg_entry g \<Longrightarrow> s \<in> S \<Longrightarrow> trace_witness_d dg cmp g S v [s]"
+| proc_entry:
+    "(cfg_entry g, EA_Enter, v) \<in> edges g \<Longrightarrow> s \<in> enter_state ` S \<Longrightarrow> trace_witness_d dg cmp g S v [s]"
 | edge: "(u, a, v) \<in> edges g \<Longrightarrow> trace_witness_d dg cmp g S u tr
          \<Longrightarrow> edge_step a (last tr) = Some s'
          \<Longrightarrow> trace_witness_d dg cmp g S v (tr @ [s'])"
@@ -196,6 +394,55 @@ qed
 definition reaching_compat ::
   "(trace \<Rightarrow> 'd) \<Rightarrow> ('d \<Rightarrow> 'd \<Rightarrow> bool) \<Rightarrow> 'd \<Rightarrow> cfg \<Rightarrow> store set \<Rightarrow> pp \<Rightarrow> trace set" where
   "reaching_compat dg cmp d g S v = {tr \<in> cfg_collect_trace g S v. cmp (dg tr) d}"
+
+lemma trace_witness_d_edges:
+  assumes path: "trace_edges g u tr v"
+  assumes start: "u = cfg_entry g"
+  assumes init: "hd tr \<in> S"
+  shows "trace_witness_d dg cmp g S v tr"
+  using path start init
+proof (induction rule: trace_edges.induct)
+  case (single v s)
+  then show ?case by (intro trace_witness_d.entry) auto
+next
+  case (step u tr v a w s')
+  have tr_ne: "tr \<noteq> []"
+    using step.hyps(1) by (rule trace_edges_nonempty)
+  have prev: "trace_witness_d dg cmp g S v tr"
+    using step.IH step.prems(1,2) tr_ne by simp
+  show ?case
+    using trace_witness_d.edge[OF step.hyps(2) prev step.hyps(3)] by simp
+qed
+
+lemma trace_witness_d_proc_edges:
+  assumes enter: "(cfg_entry g, EA_Enter, pe) \<in> edges g"
+  assumes path: "trace_edges g u tr v"
+  assumes start: "u = pe"
+  assumes init: "hd tr \<in> enter_state ` S"
+  shows "trace_witness_d dg cmp g S v tr"
+  using path start init
+proof (induction rule: trace_edges.induct)
+  case (single v s)
+  then show ?case using enter by (intro trace_witness_d.proc_entry) auto
+next
+  case (step u tr v a w s')
+  have tr_ne: "tr \<noteq> []"
+    using step.hyps(1) by (rule trace_edges_nonempty)
+  have prev: "trace_witness_d dg cmp g S v tr"
+    using step.IH step.prems(1,2) tr_ne by simp
+  show ?case
+    using trace_witness_d.edge[OF step.hyps(2) prev step.hyps(3)] by simp
+qed
+
+lemma trace_witness_d_combineI:
+  assumes comb: "(c, ex, v) \<in> combines g"
+  assumes caller: "trace_witness_d dg cmp g S c tau"
+  assumes callee: "trace_witness_d dg cmp g S ex rho"
+  assumes enter: "hd rho = enter_state (last tau)"
+  assumes compat: "cmp (dg tau) (dg rho)"
+  assumes ret: "r = <last tau|last rho>"
+  shows "trace_witness_d dg cmp g S v (tau @ tl rho @ [r])"
+  using assms trace_witness_d.combine by fastforce
 
 lemma reaching_compat_subset:
   "reaching_compat dg cmp d g S v \<subseteq> cfg_collect_trace g S v"
